src/SDK/Keyring/Defs.dfy
@@ -15,7 +15,7 @@ include "../AlgorithmSuite.dfy"
 
     method OnEncrypt(algorithmSuiteID: Materials.AlgorithmSuite.ID,
                      encryptionContext: Materials.EncryptionContext,
-                     plaintextDataKey: Option<seq<uint8>>) returns (res: Result<Option<Materials.ValidDataKey>>)
+                     plaintextDataKey: Option<seq<uint8>>) returns (res: Result<Option<Materials.ValidDataKeyMaterials>>)
       requires Valid()
       requires plaintextDataKey.Some? ==> algorithmSuiteID.ValidPlaintextDataKey(plaintextDataKey.get)
       ensures Valid()
